revisions to expr, adding syntactic types.

theories/RecordTableaux.v
@@ -1,66 +1,52 @@
 Require Import Coq.Lists.List.
 Require Import ExtLib.Tactics.
+Require Import SemanticQuery.Types.
+Require Import SemanticQuery.Expr.
 Require Import SemanticQuery.Tables.
 
 Set Implicit Arguments.
 Set Strict Implicit.
 
 Section with_tables.
-  Variable tbls : list row_type.
+  Variable scheme : list type. (** A bit odd **)
 
-  Definition binds_type : list row_type -> Type :=
-    hlist (fun x => member x tbls).
+  Definition binds_type : list type -> Type :=
+    hlist (fun x => member x scheme).
 
-  Definition guard_type (vars : list row_type) : Type :=
-    {T : dec_type & expr vars T & expr vars T}.
+  Definition guard_type (vars : list type) : Type :=
+    expr vars Bool.
 
-  Definition filter_type (vars : list row_type) : Type :=
+  Definition filter_type (vars : list type) : Type :=
     list (guard_type vars).
 
-  Definition ret_type (vars : list row_type) (result : list dec_type) : Type :=
+  Definition ret_type (vars : list type) (result : list type) : Type :=
     hlist (expr vars) result.
 
   Record tableaux :=
-  { types : list row_type
+  { types : list type
   ; binds : binds_type types
   ; filter : filter_type types
   }.
 
-  Record query (t : list dec_type) : Type :=
+  Record query (t : list type) : Type :=
   { tabl : tableaux
   ; ret  : ret_type tabl.(types) t
   }.
 
-  Fixpoint bindD {ts : list row_type} (names : binds_type ts)
-    : hlist table tbls -> list (hlist row ts) :=
-    match names in hlist _ ts return hlist table tbls -> list (hlist row ts) with
+  Fixpoint bindD {ts : list type} (names : binds_type ts)
+  : DB scheme -> list (hlist typeD ts) :=
+    match names in hlist _ ts return DB scheme -> list (hlist typeD ts) with
     | Hnil => fun _ => Hnil :: nil
     | Hcons _ _ n names => fun tbls =>
                              cross (fun a b => Hcons a b) (hlist_get n tbls) (bindD names tbls)
     end.
 
-  Fixpoint exprD {T} {ls} (e : expr ls T) {struct e} : hlist row ls -> type T :=
-    match e in expr _ T return hlist row ls -> type T with
-    | Proj _ _ v c => fun vars => hlist_get c (hlist_get v vars)
-    end.
-
-  Definition guardD {ts : list row_type} (g : guard_type ts)
-  : hlist row ts -> bool :=
-    let '(existT2 t f1 f2) := g in
-    let f1 := exprD f1 in
-    let f2 := exprD f2 in
-    fun rows =>
-      match t.(eq_dec) (f1 rows) (f2 rows) with
-      | left _ => true
-      | right _ => false
-      end.
-
-  Fixpoint filterD {ts : list row_type} (f : filter_type ts)
-  : hlist row ts -> bool :=
+  Fixpoint filterD {ts : list type} (f : filter_type ts)
+  : exprT ts bool :=
     match f with
     | nil => fun _ => true
     | f :: fs =>
-      let fD := guardD f in
+      let fD := exprD f in
       let rD := filterD fs in
       fun rows => if fD rows then rD rows else false
     end.
@@ -68,7 +54,8 @@ Section with_tables.
   (** The return type here is a bit odd. I'm just gluing the rows together as an hlist.
    ** Queries seem more natural.
    **)
-  Definition tableauxD (t : tableaux) : hlist table tbls -> list (hlist row t.(types)) :=
+  Definition tableauxD (t : tableaux)
+  : DB scheme -> list (hlist typeD t.(types)) :=
     let all := bindD t.(binds) in
     let keep := filterD t.(filter) in
     fun tbls => List.filter keep (all tbls).
@@ -89,28 +76,15 @@ Section with_tables.
       end.
   End hlist_build2.
 
-  Definition retD {ts ts'} (rt : ret_type ts ts') : hlist row ts -> row ts' :=
+  Definition retD {ts ts'} (rt : ret_type ts ts')
+  : exprT ts (Env ts') :=
     fun vars => hlist_map (fun t e => exprD e vars) rt.
 
   Definition queryD ts (q : query ts)
-  : hlist table tbls -> list (hlist type ts) :=
+  : DB scheme -> list (hlist typeD ts) :=
     fun tbls => List.map (retD q.(ret)) (tableauxD q.(tabl) tbls).
 
-  Fixpoint expr_subst {vars vars'} (f :forall {x}, member x vars -> member x vars') (T : _)
-           (e : expr vars T) {struct e} : expr vars' T :=
-    match e in expr _ T return expr vars' T with
-    | Proj _ _ v c => Proj (f v) c
-    end.
-  Arguments expr_subst {_ _} _ _ _.
-
-  Definition guard_subst {vars vars'} (f : forall {T}, expr vars T -> expr vars' T)
-             (x : guard_type vars)
-    : guard_type vars' :=
-    match x with
-    | existT2 T x1 x2 =>
-      @existT2 _ _ _ T (f x1) (f x2)
-    end.
-
+  (** TODO: Move these **)
   Definition list_set_subset {T} (a b : list T) : Prop :=
     forall x, In x a -> In x b.
 
@@ -124,18 +98,18 @@ Section with_tables.
     2) t1 |- p = q in t1 implies t2 |- h(p) = h(q)
     3) return E in t1 and return E' in t2 implies t2 |- h(E) = E'
    *)
-  Definition types_homomorphism (ts1 ts2 : list row_type) : Type :=
-    forall x : row_type, member x ts1 -> member x ts2.
-  Definition binds_homomorphism {ts1 ts2 : list row_type}
+  Definition types_homomorphism (ts1 ts2 : list type) : Type :=
+    forall x : type, member x ts1 -> member x ts2.
+  Definition binds_homomorphism {ts1 ts2 : list type}
              (h : types_homomorphism ts1 ts2)
-             (b1 : hlist (fun x => member x tbls) ts1)
-             (b2 : hlist (fun x => member x tbls) ts2) : Type :=
+             (b1 : hlist (fun x => member x scheme) ts1)
+             (b2 : hlist (fun x => member x scheme) ts2) : Type :=
     forall t (x : member t _), hlist_get x b1 = hlist_get (h _ x) b2.
-  Definition filter_homomorphism {ts1 ts2 : list row_type}
+  Definition filter_homomorphism {ts1 ts2 : list type}
              (h : types_homomorphism ts1 ts2)
              (f1 : list (guard_type ts1))
              (f2 : list (guard_type ts2)) : Type :=
-    forall x, filterD (map (guard_subst (expr_subst h)) f1) x = filterD f2 x.
+    forall x, filterD (map (expr_subst h) f1) x = filterD f2 x. (** TODO: this is too strong **)
 
   Record tableaux_homomorphism (t1 t2 : tableaux) : Type :=
   { vars_mor : types_homomorphism t1.(types) t2.(types)
@@ -143,6 +117,231 @@ Section with_tables.
   ; filterOk : filter_homomorphism vars_mor t1.(filter) t2.(filter) (** 2 **)
   }.
 
+  Record query_homomorphism ts (q1 q2 : query ts) : Type :=
+  { th : tableaux_homomorphism q1.(tabl) q2.(tabl)
+  ; retOk : forall r, filterD (map (expr_subst th.(vars_mor)) q1.(tabl).(filter)) r = true ->
+              retD (hlist_map (fun T (x : expr q1.(tabl).(types) T) =>
+                                 expr_subst th.(vars_mor) x) q1.(ret)) r =
+              retD q2.(ret) r
+  }.
+
+  Definition related {T} {F} {ts1 ts2 : list T}
+             (h : forall x : T, member x ts1 -> member x ts2)
+             (b1 : hlist F ts1)
+             (b2 : hlist F ts2) : Prop :=
+    forall t (m : member t ts1),
+      hlist_get m b1 = hlist_get (h _ m) b2.
+
+  Lemma In_bindD_hlist_get
+    : forall (l : type) (ts2 : list type) (tbl_data : DB scheme)
+             (b2 : hlist (fun x : type => member x scheme) ts2)
+             (x : Env ts2)
+             (m : member l ts2),
+      In x (bindD b2 tbl_data) ->
+      In (hlist_get m x) (hlist_get (hlist_get m b2) tbl_data).
+  Proof.
+    induction b2.
+    { simpl. intros. inversion m. }
+    { simpl. intros.
+      eapply In_cross in H. forward_reason.
+      subst.
+      destruct (member_case m); forward_reason.
+      { subst. simpl. auto. }
+      { subst. simpl. eauto. } }
+  Qed.
+
+  Lemma bindD_subset
+    : forall ts1 (b1 : hlist (fun x => member x scheme) ts1)
+             ts2 (b2 : hlist (fun x => member x scheme) ts2),
+      forall tbl_data x,
+        In x (bindD b2 tbl_data) ->
+        forall (h : types_homomorphism ts1 ts2),
+          binds_homomorphism h b1 b2 ->
+          exists y,
+            related h y x /\
+            In y (bindD b1 tbl_data).
+  Proof.
+    induction b1.
+    { intros. exists Hnil.
+      simpl. split; eauto.
+      red. clear. intros. inversion m. }
+    { simpl. intros.
+      setoid_rewrite In_cross.
+      specialize (IHb1 _ _ _ _ H (fun t m => h t (MN _ m))).
+      match goal with
+      | H : ?X -> _ |- _ =>
+        cut X;
+          [ let H' := fresh in
+            intro H' ; specialize (H H') | ]
+      end.
+      { forward_reason.
+        exists (Hcons (hlist_get (h _ (MZ _ _)) x) x0).
+        split.
+        { red. intros.
+          destruct (member_case m).
+          { destruct H3. subst. simpl. reflexivity. }
+          { forward_reason. subst. simpl. eauto. } }
+        { do 2 eexists; split; eauto.
+          red in X. red in H0.
+          specialize (X l (MZ l ls)).
+          simpl in X. subst.
+          eauto using In_bindD_hlist_get. } }
+      { revert X. clear. unfold binds_homomorphism.
+        intros. eapply (X t (MN _ x)). } }
+  Qed.
+
+  (** TODO: Move **)
+  Lemma related_exprD_subst_expr
+  : forall (types0 types1 : list type)
+           (vars_mor0 : types_homomorphism types1 types0)
+           (x0 : Env types0) (x : Env types1),
+      related vars_mor0 x x0 ->
+      forall x1 (e : expr types1 x1),
+        exprD (expr_subst vars_mor0 e) x0 = exprD e x.
+  Proof.
+    induction e.
+    { simpl. red in H. symmetry. eapply H. }
+    { simpl. rewrite IHe. reflexivity. }
+    { simpl. rewrite IHe1. rewrite IHe2. reflexivity. }
+  Qed.
+
+  Lemma related_filterD_subst_test
+    : forall (ts : list type) (q1 : query ts) (tabl0 : tableaux)
+             (vars_mor0 : types_homomorphism (types tabl0) (types (tabl q1)))
+             (x0 : Env q1.(tabl).(types)) (x : Env tabl0.(types)),
+      related vars_mor0 x x0 ->
+      forall l : filter_type tabl0.(types),
+        filterD l x = filterD (map (expr_subst vars_mor0) l) x0.
+  Proof.
+    induction l; simpl; auto.
+    { erewrite related_exprD_subst_expr by eauto.
+      rewrite <- IHl.
+      reflexivity. }
+  Qed.
+
+  Lemma retD_related
+    : forall (types1 types0 : list type)
+             (x0 : Env types1) (x : Env types0)
+             (vars_mor0 : types_homomorphism types0 types1),
+      related vars_mor0 x x0 ->
+      forall (ts : list type)
+             (ret0 : hlist (expr types0) ts),
+        retD ret0 x =
+        retD
+          (hlist_map
+             (fun T (x1 : expr types0 T) => expr_subst vars_mor0 x1)
+             ret0) x0.
+  Proof.
+    induction ret0; simpl; auto.
+    f_equal.
+    { erewrite related_exprD_subst_expr; eauto. }
+    { eassumption. }
+  Qed.
+
+  Lemma homomorphism_subset ts
+    : forall q1 q2,
+      @query_homomorphism ts q2 q1 ->
+      forall tbls,
+        list_set_subset (queryD q1 tbls) (queryD q2 tbls).
+  Proof.
+    unfold queryD, tableauxD.
+    destruct 1. red.
+    intros.
+    eapply List.in_map_iff in H.
+    eapply List.in_map_iff.
+    forward_reason.
+    eapply List.filter_In in H0.
+    setoid_rewrite List.filter_In.
+    forward_reason.
+    eapply bindD_subset in H0.
+    2: eapply bindsOk.
+    revert H0; instantiate (4 := th0); intro H0.
+    subst. forward_reason.
+    destruct th0; simpl in *.
+    exists x. split; [ | split ].
+    { rewrite <- retOk0.
+      { destruct q2. simpl in *. clear - H.
+        destruct q1. simpl in *. clear - H.
+        destruct tabl0; destruct tabl1. simpl in *.
+        eauto using retD_related. }
+      { rewrite <- H1.
+        red in filterOk0.
+        rewrite <- filterOk0. reflexivity. } }
+    { assumption. }
+    { red in filterOk0. clear retOk0 bindsOk0.
+      rewrite <- filterOk0 in H1.
+      rewrite <- H1.
+      destruct q2. simpl in *.
+      eapply related_filterD_subst_test; eauto. }
+  Qed.
+
+  Theorem bihomomorphism_equal ts
+    : forall q1 q2,
+      @query_homomorphism ts q1 q2 ->
+      @query_homomorphism ts q2 q1 ->
+      forall tbls,
+        list_set_equiv (queryD q1 tbls) (queryD q2 tbls).
+  Proof.
+    unfold list_set_equiv. intros; eauto using homomorphism_subset.
+  Qed.
+
+  (** Embedded Dependencies **)
+  (***************************)
+  Record embedded_dependency :=
+  { front_types : list type
+  ; front_binds : binds_type front_types
+  ; front_filter : filter_type front_types
+  ; back_types : list type
+  ; back_binds : binds_type back_types
+  ; back_filter : filter_type (front_types ++ back_types)
+  }.
+
+  (** TODO(gmalecha): I should make sure that I am being consistent about
+   ** the order of binders
+   **)
+  Definition embedded_dependencyD (ed : embedded_dependency)
+  : DB scheme -> Prop :=
+    let front :=
+        tableauxD {| types := ed.(front_types)
+                   ; binds := ed.(front_binds)
+                   ; filter := ed.(front_filter)
+                   |}
+    in
+    let back :=
+        let all := bindD ed.(back_binds) in
+        let keep := filterD ed.(back_filter) in
+        fun tbls base => List.filter keep (List.map (fun x => hlist_app base x) (all tbls))
+    in
+    fun tbls =>
+      forall res,
+        In res (front tbls) ->
+        exists val,
+          In val (back tbls res).
+
+  Definition ed_front (ed : embedded_dependency) : tableaux :=
+  {| types := ed.(front_types)
+   ; binds := ed.(front_binds)
+   ; filter := ed.(front_filter)
+  |}.
+
+  Fixpoint member_weaken {T} {ls : list T} {x} ls' (m : member x ls)
+  : member x (ls ++ ls') :=
+    match m in member _ ls return member x (ls ++ ls') with
+    | MZ _ => MZ _ _
+    | MN _ _ m' => MN _ (member_weaken ls' m')
+    end.
+
+  Fixpoint filter_weaken vars rt
+  : filter_type vars -> filter_type (rt :: vars) :=
+    List.map (fun x => expr_lift (rt::nil) x).
+
+  Definition ed_back (ed : embedded_dependency) : tableaux :=
+  {| types := ed.(front_types) ++ ed.(back_types)
+   ; binds := hlist_app ed.(front_binds) ed.(back_binds)
+   ; filter := List.map (expr_subst (fun t x => member_weaken ed.(back_types) x)) ed.(front_filter) ++ ed.(back_filter)
+  |}.
+
+  (** Search for homomorphisms **)
   Fixpoint member_eq' {T} {a b : T} {ls} (m1 : member a ls) (m2 : member b ls)
   : option { pf : b = a | m1 = match pf in _ = X return member X ls with
                                | eq_refl => m2
@@ -213,68 +412,68 @@ Section with_tables.
        end m2).
 
 
-    Fixpoint find_matching {T} {vs} (t : member T tbls)
-             (ts : hlist (fun rt => member rt tbls) vs)
-    : list { t' : member _ vs | hlist_get t' ts = t } :=
-      match ts in hlist _ vs
-            return list { t' : member _ vs | hlist_get t' ts = t }
+  Fixpoint find_matching {T} {vs} (t : member T scheme)
+           (ts : hlist (fun rt => member rt scheme) vs)
+  : list { t' : member _ vs | hlist_get t' ts = t } :=
+    match ts in hlist _ vs
+          return list { t' : member _ vs | hlist_get t' ts = t }
+    with
+    | Hnil => nil
+    | Hcons l ls m h =>
+      match member_eq' t m with
+      | None => nil
+      | Some (exist pf pf') =>
+        @exist _ _ match pf in _ = X return member X (l :: ls) with
+                   | eq_refl => MZ _ _
+                   end
+               (match pf as pf in _ = X
+                      return forall t : member X scheme,
+                    t = match pf in (_ = X') return (member X' scheme) with
+                        | eq_refl => m
+                        end ->
+                    hlist_get
+                      match pf in (_ = X') return (member X' (l :: ls)) with
+                      | eq_refl => MZ l ls
+                      end (Hcons m h) = t
+                with
+                | eq_refl => fun _ => @eq_sym _ _ _
+                end t pf') :: nil
+      end ++ List.map (fun x : {t' : member T ls | hlist_get t' h = t} =>
+                         let '(exist a b) := x in
+                         @exist _ (fun x => hlist_get x (Hcons m h) = t)
+                                (MN _ a) b) (@find_matching T ls t h)
+    end.
+
+  Definition types_homomorphism_nil ts2 : types_homomorphism nil ts2 :=
+    fun _ m =>
+      match m in member _ X return match X with
+                                   | nil => member _ ts2
+                                   | _ :: _ => unit
+                                   end
       with
-      | Hnil => nil
-      | Hcons l ls m h =>
-        match member_eq' t m with
-        | None => nil
-        | Some (exist pf pf') =>
-          @exist _ _ match pf in _ = X return member X (l :: ls) with
-                     | eq_refl => MZ _ _
-                     end
-                 (match pf as pf in _ = X
-                        return forall t : member X tbls,
-                      t = match pf in (_ = X') return (member X' tbls) with
-                          | eq_refl => m
-                          end ->
-                      hlist_get
-                        match pf in (_ = X') return (member X' (l :: ls)) with
-                        | eq_refl => MZ l ls
-                        end (Hcons m h) = t
-                  with
-                  | eq_refl => fun _ => @eq_sym _ _ _
-                  end t pf') :: nil
-        end ++ List.map (fun x : {t' : member T ls | hlist_get t' h = t} =>
-                           let '(exist a b) := x in
-                           @exist _ (fun x => hlist_get x (Hcons m h) = t)
-                                  (MN _ a) b) (@find_matching T ls t h)
+      | MZ _ => tt
+      | MN _ _ _ => tt
       end.
 
-    Definition types_homomorphism_nil ts2 : types_homomorphism nil ts2 :=
-      fun _ m =>
-        match m in member _ X return match X with
-                                     | nil => member _ ts2
-                                     | _ :: _ => unit
-                                     end
-        with
-        | MZ _ => tt
-        | MN _ _ _ => tt
-        end.
+  Definition binds_homomorphism_nil ts2 (h : types_homomorphism nil ts2)
+             (b1 : hlist (fun x : type => member x scheme) nil)
+             (b2 : hlist (fun x : type => member x scheme) ts2)
+  : @binds_homomorphism nil ts2 h b1 b2 :=
+    fun t x =>
+      match x as y in member _ X
+            return match X with
+                   | nil => hlist_get x b1 = hlist_get (h t x) b2
+                   | _ :: _ => unit
+                   end
+      with
+      | MZ _ => tt
+      | MN _ _ _ => tt
+      end.
 
-    Definition binds_homomorphism_nil ts2 (h : types_homomorphism nil ts2)
-               (b1 : hlist (fun x : row_type => member x tbls) nil)
-               (b2 : hlist (fun x : row_type => member x tbls) ts2)
-    : @binds_homomorphism nil ts2 h b1 b2 :=
-      fun t x =>
-        match x as y in member _ X
-              return match X with
-                     | nil => hlist_get x b1 = hlist_get (h t x) b2
-                     | _ :: _ => unit
-                     end
-        with
-        | MZ _ => tt
-        | MN _ _ _ => tt
-        end.
-
-    Section foo.
-    Let combine ts2 (b2 : hlist (fun x : row_type => member x tbls) ts2)
-        (l : row_type) (ls : list row_type) (m : member l tbls)
-        (bs1 : hlist (fun x : row_type => member x tbls) ls)
+  Section _combine.
+    Let combine ts2 (b2 : hlist (fun x : type => member x scheme) ts2)
+        (l : type) (ls : list type) (m : member l scheme)
+        (bs1 : hlist (fun x : type => member x scheme) ls)
         (m' : member l ts2) (pf' : hlist_get m' b2 = m)
         (th' : types_homomorphism ls ts2)
         (bh' : binds_homomorphism th' bs1 b2)
@@ -326,8 +525,8 @@ Section with_tables.
 
 
     Fixpoint all_bind_homomorphisms {ts1 ts2}
-             (b1 : hlist (fun x : row_type => member x tbls) ts1)
-             (b2 : hlist (fun x : row_type => member x tbls) ts2)
+             (b1 : hlist (fun x : type => member x scheme) ts1)
+             (b2 : hlist (fun x : type => member x scheme) ts2)
     : list { h : types_homomorphism ts1 ts2
            & @binds_homomorphism ts1 ts2 h b1 b2 } :=
       match b1 in hlist _ ts1
@@ -345,10 +544,11 @@ Section with_tables.
               (find_matching m b2)
               (all_bind_homomorphisms bs1 b2)
       end.
-    End foo.
+  End _combine.
 
-    Fixpoint expr_eq {vs} {t} (e1 e2 : expr vs t) {struct e1}
-    : option (e1 = e2).
+(*
+  Fixpoint expr_eq {vs} {t} (e1 e2 : expr vs t) {struct e1}
+  : option (e1 = e2).
     refine
       (match e1 as e1 in expr _ t1 , e2 as e2 in expr _ t2
              return forall pf : t1 = t2, option (match pf in _ = X return expr _ X with
@@ -356,51 +556,51 @@ Section with_tables.
                                                  end = e2)
        with
        | Proj _ _ t1 f1 , Proj _ _ t2 f2 => fun pf =>
-         _ 
+                                              _ 
        end eq_refl).
     refine
       (match pf as pf in _ = y
-            return forall f2 : member y r0,
+             return forall f2 : member y r0,
            option (match pf in (_ = X) return (expr vs X) with
                    | eq_refl => Proj t1 f1
                    end = Proj t2 f2)
-      with
-      | eq_refl => fun f2 =>
-        match member_eq' t1 t2 with
-        | None => None
-        | Some (exist pf pf') =>
-          match member_eq' f1 match pf in _ = X return member _ X with
-                             | eq_refl => f2
-                             end
-          with
-          | None => None
-          | Some (exist pf'' pf''') => Some _
-          end
-        end
-      end f2); clear pf.
+       with
+       | eq_refl => fun f2 =>
+                      match member_eq' t1 t2 with
+                      | None => None
+                      | Some (exist pf pf') =>
+                        match member_eq' f1 match pf in _ = X return member _ X with
+                                            | eq_refl => f2
+                                            end
+                        with
+                        | None => None
+                        | Some (exist pf'' pf''') => Some _
+                        end
+                      end
+       end f2); clear pf.
     destruct pf0. destruct pf'.
     f_equal. subst. clear.
     admit. (** This requires decidable equality on types **)
-    Defined.
+  Defined.
+*)
 
-    Definition check_guard {ts1} (g1 g2 : guard_type ts1)
-      : option (forall r, guardD g1 r = guardD g2 r).
-      destruct g1. destruct g2; simpl.
-    Admitted.
+  Definition check_guard {ts1} (g1 g2 : guard_type ts1)
+    : option (forall r, exprD g1 r = exprD g2 r).
+  Admitted.
 
-    Definition check_filter {ts} (f1 f2 : filter_type ts)
+  Definition check_filter {ts} (f1 f2 : filter_type ts)
     : option (forall rows, filterD f1 rows = filterD f2 rows).
-    Admitted.
+  Admitted.
 
-    Fixpoint filter_map {T U} (f : T -> option U) (ls : list T) : list U :=
-      match ls with
-      | nil => nil
-      | l :: ls =>
-        match f l with
-        | None => filter_map f ls
-        | Some x => x :: filter_map f ls
-        end
-      end.
+  Fixpoint filter_map {T U} (f : T -> option U) (ls : list T) : list U :=
+    match ls with
+    | nil => nil
+    | l :: ls =>
+      match f l with
+      | None => filter_map f ls
+      | Some x => x :: filter_map f ls
+      end
+    end.
 
   Definition find_homomorphisms (t1 t2 : tableaux)
   : list (tableaux_homomorphism t1 t2) :=
@@ -409,7 +609,7 @@ Section with_tables.
                          & binds_homomorphism h t1.(binds) t2.(binds) }) =>
                   let '(existT vm bm) := x in
                   match
-                    check_filter (map (guard_subst (expr_subst vm)) t1.(filter))
+                    check_filter (map (expr_subst vm) t1.(filter))
                                  t2.(filter)
                   with
                   | None => None
@@ -418,233 +618,5 @@ Section with_tables.
                           ; bindsOk := bm
                           ; filterOk := fh |}
                   end) xs.
-
-  Record query_homomorphism ts (q1 q2 : query ts) : Type :=
-  { th : tableaux_homomorphism q1.(tabl) q2.(tabl)
-  ; retOk : forall r, filterD (map (guard_subst (expr_subst th.(vars_mor))) q1.(tabl).(filter)) r = true ->
-              retD (hlist_map (fun T (x : expr (types q1.(tabl)) T) => expr_subst th.(vars_mor) _ x) q1.(ret)) r =
-              retD q2.(ret) r
-  }.
-
-  Definition related {ts1 ts2 : list row_type} (h : forall x : row_type, member x ts1 -> member x ts2)
-             (b1 : hlist row ts1)
-             (b2 : hlist row ts2) : Prop :=
-    forall t (m : member t ts1),
-      hlist_get m b1 = hlist_get (h _ m) b2.
-
-  Lemma In_bindD_hlist_get
-    : forall (l : row_type) (ts2 : list row_type) (tbl_data : hlist table tbls)
-             (b2 : hlist (fun x : row_type => member x tbls) ts2)
-             (x : hlist row ts2)
-             (m : member l ts2),
-      In x (bindD b2 tbl_data) ->
-      In (hlist_get m x) (hlist_get (hlist_get m b2) tbl_data).
-  Proof.
-    induction b2.
-    { simpl. intros. inversion m. }
-    { simpl. intros.
-      eapply In_cross in H. forward_reason.
-      subst.
-      destruct (member_case m); forward_reason.
-      { subst. simpl. auto. }
-      { subst. simpl. eauto. } }
-  Qed.
-
-  Lemma bindD_subset
-    : forall ts1 (b1 : hlist (fun x => member x tbls) ts1)
-             ts2 (b2 : hlist (fun x => member x tbls) ts2),
-      forall tbl_data x,
-        In x (bindD b2 tbl_data) ->
-        forall (h : types_homomorphism ts1 ts2),
-          binds_homomorphism h b1 b2 ->
-          exists y,
-            related h y x /\
-            In y (bindD b1 tbl_data).
-  Proof.
-    induction b1.
-    { intros. exists Hnil.
-      simpl. split; eauto.
-      red. clear. intros. inversion m. }
-    { simpl. intros.
-      setoid_rewrite In_cross.
-      specialize (IHb1 _ _ _ _ H (fun t m => h t (MN _ m))).
-      match goal with
-      | H : ?X -> _ |- _ =>
-        cut X;
-          [ let H' := fresh in
-            intro H' ; specialize (H H') | ]
-      end.
-      { forward_reason.
-        exists (Hcons (hlist_get (h _ (MZ _ _)) x) x0).
-        split.
-        { red. intros.
-          destruct (member_case m).
-          { destruct H3. subst. simpl. reflexivity. }
-          { forward_reason. subst. simpl. eauto. } }
-        { do 2 eexists; split; eauto.
-          red in X. red in H0.
-          specialize (X l (MZ l ls)).
-          simpl in X. subst.
-          eauto using In_bindD_hlist_get. } }
-      { revert X. clear. unfold binds_homomorphism.
-        intros. eapply (X t (MN _ x)). } }
-  Qed.
-
-  Lemma related_exprD_subst_expr
-  : forall (types0 types1 : list row_type)
-           (vars_mor0 : types_homomorphism types1 types0)
-           (x0 : hlist row types0) (x : hlist row types1),
-      related vars_mor0 x x0 ->
-      forall (x1 : dec_type) (e : expr types1 x1),
-        exprD (expr_subst vars_mor0 x1 e) x0 = exprD e x.
-  Proof.
-    induction e.
-    { simpl. red in H.
-      f_equal. symmetry. eapply H. }
-  Qed.
-
-  Lemma related_filterD_subst_test
-    : forall (ts : list dec_type) (q1 : query ts) (tabl0 : tableaux)
-             (vars_mor0 : types_homomorphism (types tabl0) (types (tabl q1)))
-             (x0 : hlist row (types (tabl q1))) (x : hlist row (types tabl0)),
-      related vars_mor0 x x0 ->
-      forall
-        l : list {T : dec_type & expr (types tabl0) T & expr (types tabl0) T},
-        filterD l x = filterD (map (guard_subst (expr_subst vars_mor0)) l) x0.
-  Proof.
-    induction l; simpl; auto.
-    { destruct a; simpl.
-      rewrite <- IHl.
-      do 2 erewrite related_exprD_subst_expr by eauto.
-      reflexivity. }
-  Qed.
-
-  Lemma retD_related
-    : forall (types1 types0 : list row_type)
-             (x0 : hlist row types1) (x : hlist row types0)
-             (vars_mor0 : types_homomorphism types0 types1),
-      related vars_mor0 x x0 ->
-      forall (ts : list dec_type)
-             (ret0 : hlist (expr types0) ts),
-        retD ret0 x =
-        retD
-          (hlist_map
-             (fun (T : dec_type) (x1 : expr types0 T) => expr_subst vars_mor0 T x1)
-             ret0) x0.
-  Proof.
-    induction ret0; simpl; auto.
-    f_equal.
-    { erewrite related_exprD_subst_expr; eauto. }
-    { eassumption. }
-  Qed.
-
-  Lemma homomorphism_subset ts
-    : forall q1 q2,
-      @query_homomorphism ts q2 q1 ->
-      forall tbls,
-        list_set_subset (queryD q1 tbls) (queryD q2 tbls).
-  Proof.
-    unfold queryD, tableauxD.
-    destruct 1. red.
-    intros.
-    eapply List.in_map_iff in H.
-    eapply List.in_map_iff.
-    forward_reason.
-    eapply List.filter_In in H0.
-    setoid_rewrite List.filter_In.
-    forward_reason.
-    eapply bindD_subset in H0.
-    2: eapply bindsOk.
-    revert H0; instantiate (4 := th0); intro H0.
-    subst. forward_reason.
-    destruct th0; simpl in *.
-    exists x. split; [ | split ].
-    { rewrite <- retOk0.
-      { destruct q2. simpl in *. clear - H.
-        destruct q1. simpl in *. clear - H.
-        destruct tabl0; destruct tabl1. simpl in *.
-        eauto using retD_related. }
-      { rewrite <- H1.
-        red in filterOk0.
-        rewrite <- filterOk0. reflexivity. } }
-    { assumption. }
-    { red in filterOk0. clear retOk0 bindsOk0.
-      rewrite <- filterOk0 in H1.
-      rewrite <- H1.
-      destruct q2. simpl in *.
-      eapply related_filterD_subst_test; eauto. }
-  Qed.
-
-  Theorem bihomomorphism_equal ts
-    : forall q1 q2,
-      @query_homomorphism ts q1 q2 ->
-      @query_homomorphism ts q2 q1 ->
-      forall tbls,
-        list_set_equiv (queryD q1 tbls) (queryD q2 tbls).
-  Proof.
-    unfold list_set_equiv. intros; eauto using homomorphism_subset.
-  Qed.
-
-  (** Embedded Dependencies **)
-  (***************************)
-  Record embedded_dependency :=
-  { front_types : list row_type
-  ; front_binds : binds_type front_types
-  ; front_filter : filter_type front_types
-  ; back_types : list row_type
-  ; back_binds : binds_type back_types
-  ; back_filter : filter_type (front_types ++ back_types)
-  }.
-
-  (** TODO(gmalecha): I should make sure that I am being consistent about
-   ** the order of binders
-   **)
-  Definition embedded_dependencyD (ed : embedded_dependency)
-  : hlist table tbls -> Prop :=
-    let front :=
-        tableauxD {| types := ed.(front_types)
-                   ; binds := ed.(front_binds)
-                   ; filter := ed.(front_filter)
-                   |}
-    in
-    let back :=
-        let all := bindD ed.(back_binds) in
-        let keep := filterD ed.(back_filter) in
-        fun tbls base => List.filter keep (List.map (fun x => hlist_app base x) (all tbls))
-    in
-    fun tbls =>
-      forall res,
-        In res (front tbls) ->
-        exists val,
-          In val (back tbls res).
-
-  Definition ed_front (ed : embedded_dependency) : tableaux :=
-  {| types := ed.(front_types)
-   ; binds := ed.(front_binds)
-   ; filter := ed.(front_filter)
-  |}.
-
-  Fixpoint member_weaken {T} {ls : list T} {x} ls' (m : member x ls)
-  : member x (ls ++ ls') :=
-    match m in member _ ls return member x (ls ++ ls') with
-    | MZ _ => MZ _ _
-    | MN _ _ m' => MN _ (member_weaken ls' m')
-    end.
-
-  Fixpoint filter_weaken vars rt
-    : filter_type vars -> filter_type (rt :: vars) :=
-    List.map (fun x =>
-                let '(existT2 t l r) := x in
-                @existT2 _ _ _ t
-                         (@expr_weaken vars rt _ l)
-                         (@expr_weaken vars rt _ r)).
-
-
-  Definition ed_back (ed : embedded_dependency) : tableaux :=
-  {| types := ed.(front_types) ++ ed.(back_types)
-   ; binds := hlist_app ed.(front_binds) ed.(back_binds)
-   ; filter := List.map (guard_subst (expr_subst (fun t x => member_weaken ed.(back_types) x))) ed.(front_filter) ++ ed.(back_filter)
-  |}.
-
 
 End with_tables.
