theories/Tables.v
@@ -4,57 +4,41 @@ Require Import ExtLib.Core.RelDec.
 Require Import ExtLib.Data.HList.
 Require Import ExtLib.Data.Member.
 Require Import ExtLib.Tactics.
+Require Import SemanticQuery.Types.
+Require Import SemanticQuery.Expr.
 
 Set Implicit Arguments.
 Set Strict Implicit.
 
-Record dec_type :=
-{ type : Type
-; eq_dec : forall a b : type, {a = b} + {a <> b}
-}.
+Definition row_type : Type := list type.
 
-Definition dec_type_from_EqDec (T : Type)
-           {ED : RelDec (@eq T)} {EDO : RelDec_Correct ED}
-: dec_type :=
-{| type := T
- ; eq_dec := fun a b : T =>
-               match a ?[ eq ] b as t return a ?[ eq ] b = t -> {a = b} + {a <> b} with
-               | true => fun pf =>
-                           left (proj1 (@rel_dec_correct _ _ _ EDO a b) pf)
-               | false => fun pf =>
-                            right (proj2 (@neg_rel_dec_correct _ _ _ EDO a b) pf)
-               end eq_refl
- |}.
-
-Arguments dec_type_from_EqDec _ {_ _}.
-
-Definition row_type : Type := list dec_type.
-
-Definition row (r : row_type) : Type := hlist type r.
+Definition row (r : row_type) : Type := typeD (Tuple r).
 
 Definition table (r : row_type) := list (row r).
 
+Definition DB (ls : list type) := hlist (fun x => list (typeD x)) ls.
+
 Module Demo.
-  Require Import ExtLib.Data.Nat.
-  Require Import ExtLib.Data.String.
+  Definition tt_names : row_type := Nat :: String :: nil.
+  Definition tt_manager : row_type := Nat :: Nat :: nil.
 
-  Definition nat_type : dec_type := dec_type_from_EqDec nat.
-  Definition string_type : dec_type := dec_type_from_EqDec string.
-
-  Definition tt_names : row_type := nat_type :: string_type :: nil.
-  Definition tt_manager : row_type := nat_type :: nat_type :: nil.
-
+(*
   Fixpoint tuple (r : row_type) : Type :=
     match r with
     | nil => unit
     | r :: rs => type r * tuple rs
     end%type.
+*)
 
-  Fixpoint Row (r : row_type) : tuple r -> hlist type r :=
-    match r as r return tuple r -> hlist type r with
+(*
+  Fixpoint Row (r : row_type) : tuple typeD r -> hlist typeD r :=
+    match r as r return tuple typeD r -> hlist typeD r with
     | nil => fun _ => Hnil
     | r :: rs => fun v => Hcons (fst v) (Row rs (snd v))
     end.
+*)
+
+  Definition Row (r : row_type) : tuple typeD r -> row r := fun x => x.
 
   Definition tbl_names : table tt_names :=
     (Row tt_names (0, ("Ryan"%string, tt))) ::
@@ -65,24 +49,13 @@ Module Demo.
     (Row tt_manager (1, (0, tt))) :: nil.
 End Demo.
 
-(** Deeply embedded expressions **)
-Inductive expr (vars : list row_type) : dec_type -> Type :=
-| Proj : forall T r, member r vars -> member T r -> expr vars T.
-
-Fixpoint expr_weaken vars rt T (e : expr vars T) {struct e}
-  : expr (rt :: vars) T :=
-  match e in @expr _ T return expr (rt :: vars) T with
-  | Proj _ _ t f => Proj (Member.MN _ t) f
-  end.
-
-
+(** Cross-product of tables **)
 Fixpoint cross {T U V : Type} (f : T -> U -> V) (ts : list T) (us : list U)
 : list V :=
   match ts with
   | nil => nil
   | t :: ts => List.map (f t) us ++ cross f ts us
   end.
-
 
 Lemma In_cross : forall {T U V} (f : T -> U -> V) us ts,
     forall x,
