theories/Expr.v
@@ -1,0 +1,75 @@
+Require Import Coq.Lists.List.
+Require Import ExtLib.Data.Member.
+Require Import ExtLib.Data.HList.
+Require Import SemanticQuery.Types.
+
+Set Implicit Arguments.
+Set Strict Implicit.
+
+(** Deeply embedded expressions **)
+Inductive expr (vars : list type) : type -> UU :=
+| Var : forall T, member T vars -> expr vars T
+| Proj : forall T r, expr vars (Tuple r) -> member T r -> expr vars T
+| Eq : forall T, expr vars T -> expr vars T -> expr vars Bool.
+
+Definition Env : list type -> U := hlist typeD.
+Definition exprT (ls : list type) (T : Type) : Type :=
+  Env ls -> T.
+
+Fixpoint exprD {vars} {t} (e : expr vars t)
+: exprT vars (typeD t) :=
+  match e in expr _ t return exprT vars (typeD t) with
+  | Var _ m => hlist_get m
+  | Proj _ r e' f =>
+    let eD := @exprD vars (Tuple r) e' in
+    let fD := tuple_get typeD f in
+    fun vs => fD (eD vs)
+  | Eq T l r =>
+    let lD := exprD l in
+    let rD := exprD r in
+    let eqD := @val_dec T in
+    fun vs => if eqD (lD vs) (rD vs) then true else false
+  end.
+
+Fixpoint member_lift {T} {t : T} (vs vs' : list T) (m : member t vs')
+: member t (vs ++ vs') :=
+  match vs as vs return member t (vs ++ vs') with
+  | nil => m
+  | v :: vs => MN _ (member_lift _ m)
+  end.
+
+Fixpoint expr_lift {T} vs vs' (e : expr vs' T) {struct e}
+: expr (vs ++ vs') T :=
+  match e in expr _ T return expr (vs ++ vs') T with
+  | Var _ m => Var (member_lift _ m)
+  | Proj _ _ a b => Proj (expr_lift _ a) b
+  | Eq T a b => Eq (expr_lift _ a) (expr_lift _ b)
+  end.
+
+Fixpoint member_weaken_app {T} {t : T} (vs vs' : list T) (m : member t vs')
+  : member t (vs' ++ vs) :=
+  match m in member _ vs' return member t (vs' ++ vs) with
+  | MZ _ => MZ _ _
+  | MN _ _ m => MN _ (member_weaken_app _ m)
+  end.
+
+Fixpoint expr_weaken_app {T} vs vs' (e : expr vs' T) {struct e}
+  : expr (vs' ++ vs) T :=
+  match e in expr _ T return expr (vs' ++ vs) T with
+  | Var _ a => Var (member_weaken_app _ a)
+  | Proj _ _ a b => Proj (expr_weaken_app _ a) b
+  | Eq T a b => Eq (expr_weaken_app _ a) (expr_weaken_app _ b)
+  end.
+
+Section _subst.
+  Context {vars vars' : list type}.
+  Variable (f :forall {x}, member x vars -> member x vars').
+
+  Fixpoint expr_subst  {T}
+           (e : expr vars T) {struct e} : expr vars' T :=
+    match e in expr _ T return expr vars' T with
+    | Var _ v => Var (f v)
+    | Proj _ _ v c => Proj (expr_subst v) c
+    | Eq T a b => Eq (expr_subst a) (expr_subst b)
+    end.
+End _subst.
