theories/Types.v
@@ -1,0 +1,96 @@
+Require Coq.Strings.String.
+Require Import Coq.Lists.List.
+Require Import ExtLib.Data.Member.
+
+Set Implicit Arguments.
+Set Strict Implicit.
+
+Let UU : Type := Type.
+Let U : UU := Type.
+
+Inductive type :=
+| Nat
+| Bool
+| String
+| Tuple : list type -> type.
+
+Section mp.
+  Variable f : type -> U.
+  Fixpoint tuple (ls : list type) : U :=
+    match ls with
+    | nil => unit
+    | List.cons l ls => (f l) * (tuple ls)
+    end%type.
+
+  Fixpoint tuple_get {ls} {t} (m : member t ls) : tuple ls -> f t :=
+    match m in member _ ls return tuple ls -> f t with
+    | MZ _ => fst
+    | MN _ _ m' =>
+      let get := tuple_get m' in
+      fun rows => get (snd rows)
+    end.
+End mp.
+
+Fixpoint typeD (t : type) : U :=
+  match t return U with
+  | Nat => nat
+  | Bool => bool
+  | String => String.string
+  | Tuple ls => tuple typeD ls
+  end.
+
+Fixpoint type_dec (a b : type) : {a = b} + {a <> b}.
+refine
+  match a as a , b as b return {a = b} + {a <> b} with
+  | Nat , Nat => left eq_refl
+  | Bool , Bool => left eq_refl
+  | String , String => left eq_refl
+  | Tuple a , Tuple b =>
+    match List.list_eq_dec type_dec a b with
+    | left pf => left (f_equal _ pf)
+    | right pf => right _
+    end
+  | _ , _ => right _
+  end; congruence.
+Defined.
+
+Definition bool_eq_dec (a b : bool) : {a = b} + {a <> b}.
+decide equality.
+Defined.
+
+Definition unit_eq_dec (a b : unit) : {a = b} + {a <> b}.
+decide equality.
+Defined.
+
+
+Definition prod_eq_dec {T U}
+            (Teq : forall a b : T, {a = b} + {a <> b})
+            (Ueq : forall a b : U, {a = b} + {a <> b})
+            (a b : T * U)
+: {a = b} + {a <> b}.
+refine
+  match a as a , b as b return {a = b} + {a <> b} with
+  | (l1,l2) , (r1,r2) =>
+    match Teq l1 r1 , Ueq l2 r2 with
+    | left _ , left _ => left _
+    | _ , _ => right _
+    end
+  end; subst; congruence.
+Defined.
+
+Fixpoint val_dec {t : type} {struct t}
+: forall (l r : typeD t), {l = r} + {l <> r} :=
+  match t as t return forall (l r : typeD t), {l = r} + {l <> r} with
+  | Nat => NPeano.Nat.eq_dec
+  | Bool => bool_eq_dec
+  | String => String.string_dec
+  | Tuple ls =>
+    (fix eq_dec ls : forall (l r : tuple typeD ls), {l = r} + {l <> r} :=
+       match ls with
+       | nil => unit_eq_dec
+       | l :: ls =>
+         let tD := @val_dec l in
+         let lD := @eq_dec ls in
+         @prod_eq_dec _ _ tD lD
+       end) ls
+  end.
